\documentclass[11pt]{article}
\usepackage{amssymb,amsmath}

\begin{document}

%<*eqExLinEqu>
\begin{equation}
    \label{equ:ExLinEqu}
    y = a_0 + a_1 x
\end{equation}
%</eqExLinEqu>

%<*eqLSEE2>
\begin{equation}
    \label{equ:LSE_E2}
    E^2 = \sum_{i=1}^{n} (y_i - y)^2
\end{equation}
%</eqLSEE2>

%<*eqLSEE2b>
\begin{equation}
    \label{equ:LSE_E2b}
    E^2 = \sum_{i=1}^{n} (y_i - (a_0 + a_1 x_i))^2
\end{equation}
%</eqLSEE2b>

%<*eqLSEPD>
\begin{align} 
    \frac{\partial E^2}{\partial a_0} &= 0 = \sum_{i=1}^{n} (-2y_i +2a_0 + 2a_1 x_i)           \label{equ:LSE_PD1} \\
    \frac{\partial E^2}{\partial a_1} &= 0 = \sum_{i=1}^{n} (-2y_i x_i +2a_0 x_i + 2a_1 x_i^2) \label{equ:LSE_PD2}
\end{align}
%</eqLSEPD>

%<*eqavgb>
\begin{equation}
    \label{equ:avgb} 
    \sum_{i=1}^{n} y_i  = \bar{y}n
\end{equation}
%</eqavgb>

%<*eqLSEsol>
\begin{equation}
    \label{equ:LSE_sol}
    0 = \bar{y} - (a_0 + 2a_1 \bar{x})
\end{equation}
%</eqLSEsol>

%<*eqLSEsolb>
\begin{equation}
    \label{equ:LSE_solb}
    0 = \bar{xy} - (a_0 \bar{x} + 2a_1 \bar{x^2})
\end{equation}
%</eqLSEsolb>

%<*eqLSEsolc>
\begin{equation}
    \label{equ:LSE_solc}
    a_0 = \bar{y} - a_1 \bar{x}
\end{equation}
%</eqLSEsolc>

%<*eqLSEsold>
\begin{equation}
    \label{equ:LSE_sold}
    a_1 = \frac{\bar{xy} - \bar{x}\bar{y}}{\bar{x^2} - \bar{x}^2}
\end{equation}
%</eqLSEsold>

%<*eqlevyGs>
\begin{equation}
    \label{equ:levy_Gs}
    G(s) = \frac{A_0 + A_1 s + A_2 s^2 + ... + A_n s^n}{B_0 + B_1 s + B_2 s^2 + ... + B_m s^m}
    ~\cite{levy}[Eq.~3]
\end{equation}
%</eqlevyGs>

%<*eqLevyL>
\begin{equation}
    \label{equ:Levy_L}
    \lambda _h = \sum_{k=0}^{m} \omega _k ^h
    ~\cite{levy}[Eq.~15]
\end{equation}
%</eqLevyL>

%<*eqLevyS>
\begin{equation}
    \label{equ:Levy_S}
    S_h = \sum_{k=0}^{m} \omega _k ^h R_k
    ~\cite{levy}[Eq.~16]
\end{equation}
%</eqLevyS>

%<*eqLevyT>
\begin{equation}
    \label{equ:Levy_T}
    T_h = \sum_{k=0}^{m} \omega _k ^h I_k
    ~\cite{levy}[Eq.~17]
\end{equation}
%</eqLevyT>

%<*eqLevyU>
\begin{equation}
    \label{equ:Levy_U}
    U_h = \sum_{k=0}^{m} \omega _k ^h (R_k ^2 + I_k ^2)
    ~\cite{levy}[Eq.~18]
\end{equation}
%</eqLevyU>

%<*eqLevyAns>
\begin{equation}
    \label{equ:Levy_Ans}
    MN = C
    ~\cite{levy}[Eq.~20]
\end{equation}
%</eqLevyAns>

%<*eqiterWeight>
\begin{equation}
    \label{equ:iter_Weight}
    W_{kL} = \frac{1}{|Q(jw_k)_{L-1}|^2}
    ~\cite{levy_iter}
\end{equation}
%</eqiterWeight>

%<*eqiterErr>
\begin{equation}
    \label{equ:iter_Err}
    E = \sum_{k=1}^{n} |\epsilon _k ^{'}|^2W_{kL}
    ~\cite{levy_iter}[Eq.~7]
\end{equation}
%</eqiterErr>

%<*eqIterL>
\begin{equation}
    \label{equ:Iter_L}
    \lambda _h = \sum_{k=0}^{m} \omega _k ^hW_{kL}
    ~\cite{levy_iter}[Eq.~9]
\end{equation}
%</eqIterL>

%<*eqIterS>
\begin{equation}
    \label{equ:Iter_S}
    S_h = \sum_{k=0}^{m} \omega _k ^h R_kW_{kL}
    ~\cite{levy_iter}[Eq.~10]
\end{equation}
%</eqIterS>

%<*eqIterT>
\begin{equation}
    \label{equ:Iter_T}
    T_h = \sum_{k=0}^{m} \omega _k ^h I_kW_{kL}
    ~\cite{levy_iter}[Eq.~11]
\end{equation}
%</eqIterT>

%<*eqIterU>
\begin{equation}
    \label{equ:Iter_U}
    U_h = \sum_{k=0}^{m} \omega _k ^h (R_k ^2 + I_k ^2)W_{kL}
    ~\cite{levy_iter}[Eq.~12]
\end{equation}
%</eqIterU>

%<*eqErrMin>
\begin{equation}
\label{equ:ErrMin}
n = min(\frac{E_{Mag}}{max(E_{Mag})} + \frac{E_{pha}}{max(E_{Pha})})
\end{equation}
%</eqErrMin>

%<*eqfullModelPoly>
\begin{equation}
    \label{equ:fullModelPoly}
    \bar{Z}(s) = \frac{a_0 + a_1s + a_2s^2 + a_3s^3}{b_0 + b_1s + b_2s^2}
\end{equation}
%</eqfullModelPoly>

%<*eqfullModelImpedance>
\begin{equation}
    \begin{split}
        \label{equ:fullModelImpedance}
        \bar{Z}(s) = \frac{(R_E + R_L) + (L_E + C_DR_DR_E + C_DR_DR_L + CR_ER_L + C_DR_ER_L)s}{1 + (C_DR_D + CR_L + C_DR_L)s + CC_DR_DR_Ls^2} \\ 
        + \frac{(C_DL_ER_D + CL_ER_L + C_DL_ER_L + CC_DR_DR_ER_L)s^2 + CC_DL_ER_DR_Ls^3}{1 + (C_DR_D + CR_L + C_DR_L)s + CC_DR_DR_Ls^2}
    \end{split}
\end{equation}
%</eqfullModelImpedance>

%<*eqfullModelM>
\begin{equation}
    \label{equ:fullModel_M}
    M = 
    \begin{bmatrix}
        \lambda _0 & 0          & -\lambda _2 & 0           &  T_1    & S_2 \\
        0          & \lambda _2 & 0           & -\lambda _4 & -S_2    & T_3 \\
        \lambda _2 & 0          & -\lambda _4 & 0           &  T_3    & S_4 \\
        0          & \lambda _4 & 0           & -\lambda _6 & -S_4    & T_5 \\
        T_1        & -S_2       & -T_3        &  S_4        &  U_2    & 0   \\
        S_2        &  T_3       & -S_4        & -T_5        &  0      & U_4
    \end{bmatrix}
\end{equation}
%</eqfullModelM>

%<*eqLevyNC>
\begin{multicols}{2}
    \begin{equation}
        \label{equ:Levy_N}
        N = 
        \begin{bmatrix}
            A_0 \\
            A_1 \\
            A_2 \\
            A_3 \\
            \vdots \\
            B_1 \\
            B_2 \\
            B_3 \\
            \vdots
        \end{bmatrix}
        ~\cite{levy}[Eq.~21b]
    \end{equation}
\par
    \begin{equation}
        \label{equ:Levy_C}
        C = 
        \begin{bmatrix}
            S_0 \\
            T_1 \\
            S_2 \\
            T_3 \\
            \vdots \\
            0   \\
            U_2 \\
            0   \\
            \vdots
        \end{bmatrix}
        ~\cite{levy}[Eq.~21c]
    \end{equation}
\end{multicols}
%</eqLevyNC>

%<*eqFullModelN>
\begin{multicols}{2}
    \begin{equation}
        \label{equ:fullModel_N}
        N = 
        \begin{bmatrix}
            A_0 \\
            A_1 \\
            A_2 \\
            A_3 \\
            B_1 \\
            B_2
        \end{bmatrix}
    \end{equation}
\par
    \begin{equation}
        \label{equ:fullModel_C}
        C = 
        \begin{bmatrix}
            S_0 \\
            T_1 \\
            S_2 \\
            T_3 \\
            0   \\
            U_2
        \end{bmatrix}
    \end{equation}
\end{multicols}
%</eqFullModelN>

%<*eqFullModelBadOut>
\begin{multicols}{2}
    \begin{equation}
        \label{equ:fullModel_BadOutputCoeff}
        \begin{split}
             a_0 &= 5.9991E^{+03} \\
             a_1 &= 1.7934E^{-04} \\
             a_2 &= 3.3158E^{-12} \\
             a_3 &= 6.8295E^{-22} \\
             b_0 &= 1.0000        \\
             b_1 &= 5.9057E^{-03} \\
             b_2 &= 1.4067E^{-12}
        \end{split}
    \end{equation}
\par
    \begin{equation}
        \label{equ:fullModel_BadOutputParams}
        \begin{split}
            C &= -8.2563E^{-10} \\
            R_E &=  3.1886E^{-01} \\
            L_E &=  4.8551E^{-10} \\
            R_L &=  4.8551E^{-10} \\
            C_D &=  9.8536E^{-07} \\
            R_D &= -2.8824E^{-01}
        \end{split}
    \end{equation}
\end{multicols}
%</eqFullModelBadOut>

%<*eqFullModelBadIn>
\begin{multicols}{2}
    \mbox{}\vfill
    \begin{equation}
        \label{equ:fullModel_BadInputCoeff}
        \begin{split}
            &a_0 = 1 \\
            &a_1 = 1 \\
            &a_2 = 1 \\
            &a_3 = 1 \\
            &b_0 = 1 \\
            &b_1 = 0 \\
            &b_2 = 0
        \end{split}
    \end{equation}
\par
    \mbox{}\vfill
    \columnbreak
\par
    \mbox{}\vfill
    \begin{equation}
        \label{equ:fullModel_BadInputParams}
        \begin{split}
             C   &= INF \\
             R_E &= INF \\
             L_E &= INF \\
             R_L &= IND \\
             C_D &= IND \\
             R_D &= IND \\
        \end{split}
    \end{equation}
    \mbox{}\vfill
\end{multicols}
%</eqFullModelBadIn>

%<*eqFullModelGoodIn>
\begin{multicols}{2}
    \mbox{}\vfill
    \begin{equation}
        \label{equ:fullModel_GoodInputCoeff}
        \begin{split}
             a_0 &= 2 \\
             a_1 &= 5 \\
             a_2 &= 4 \\
             a_3 &= 1 \\
             b_0 &= 1 \\
             b_1 &= 3 \\
             b_2 &= 1
        \end{split}
    \end{equation}
\par
    \mbox{}\vfill
    \columnbreak
\par
    \mbox{}\vfill
    \begin{equation}
        \label{equ:fullModel_GoodInputParams}
        \begin{split}
             C   &= 1 \\
             R_E &= 1 \\
             L_E &= 1 \\
             R_L &= 1 \\
             C_D &= 1 \\
             R_D &= 1 \\
        \end{split}
    \end{equation}
    \mbox{}\vfill
\end{multicols}
%</eqFullModelGoodIn>

\end{document}

